generic/Zeta.AppSimulate.fsti
@@ -1,0 +1,87 @@
+module Zeta.AppSimulate
+
+open Zeta.App
+
+module S = FStar.Seq
+module SA = Zeta.SeqAux
+
+(* An invocation of an application function *)
+type appfn_call (aprm: app_params) = {
+
+  (* id of the function *)
+  fid_call: appfn_id aprm;
+
+  (* arguments of the function *)
+  arg: appfn_arg fid_call;
+
+  (* the read records of the function call *)
+  inp: appfn_rs_t fid_call;
+}
+
+(* the (full) application state  *)
+let app_state (adm: app_data_model) = (k: app_key adm) -> app_value_nullable adm
+
+(* update the value for a record *)
+let update #adm (st: app_state adm) (k: app_key adm) (v: app_value_nullable adm): app_state adm =
+  fun k' -> if k' = k then v
+          else st k'
+
+(* if a sequence has distinct keys, then a prefix of the sequence also has this property *)
+val prefix_of_distinct_distinct
+  (#adm: app_data_model)
+  (sk: S.seq (app_record adm) {distinct_keys #adm sk})
+  (i: nat { i <= S.length sk }) :
+  Lemma (ensures (let sk' = SA.prefix sk i in
+                  distinct_keys #adm sk'))
+        [SMTPat (SA.prefix sk i)]
+
+(* update the state with new values for a sequence of keys (specified as a record) *)
+let rec update_seq #adm
+  (st: app_state adm)
+  (inp: S.seq (app_record adm) {distinct_keys #adm inp})
+  (ws: S.seq (app_value_nullable adm) {S.length ws = S.length inp})
+  : Tot (app_state adm)
+  (decreases (S.length inp)) =
+
+  let n = S.length inp in
+  if n = 0 then st
+  else
+    let inp' = SA.prefix inp (n - 1) in
+    let ws' = SA.prefix ws (n - 1) in
+    let st = update_seq st inp' ws' in
+    let k,_ = S.index inp (n - 1) in
+    let v = S.index ws (n - 1) in
+    update st k v
+
+(* simulate a single step of an app state transition. return None on failure *)
+let simulate_step #aprm (fncall: appfn_call aprm) (st: app_state aprm.adm):
+  option ( app_state aprm.adm & appfn_res fncall.fid_call) =
+  let fn = appfn fncall.fid_call in
+  let rc,res,ws = fn fncall.arg fncall.inp in
+  if rc = Fn_failure then None
+  else Some (update_seq st fncall.inp ws, res)
+
+(* the result of a function. We need this type since the we cannot simply define a
+ * seq (result), since the result type depends on the function id.
+ *)
+type appfn_call_res (aprm: app_params) =
+  | FnRes: fid_res: appfn_id aprm -> res: appfn_res fid_res -> appfn_call_res aprm
+
+(* initial state of the application *)
+let init_app_state (adm: app_data_model): app_state adm =
+  fun _ -> Null
+
+let consistent #aprm (call_seq: S.seq (appfn_call aprm)) (res_seq: S.seq (appfn_call_res aprm)) =
+  S.length call_seq = S.length res_seq /\
+  (forall (i: SA.seq_index call_seq).
+    {:pattern ((S.index call_seq i).fid_call = (S.index res_seq i).fid_res)}
+    (S.index call_seq i).fid_call = (S.index res_seq i).fid_res)
+
+let rec simulate #aprm (fs: S.seq (appfn_call aprm)):
+  Tot (or: option (app_state aprm.adm & S.seq (appfn_call_res aprm))
+        {Some? or ==> (let _,rs = Some?.v or in
+                       consistent fs rs)})
+  (decreases (S.length fs)) =
+  let n = S.length fs in
+
+  admit()
